monadproofs/proofs/demo2prf.v
@@ -1,9 +1,9 @@
 Require Import monad.proofs.demo2.
-
-Require Import monad.proofs.misc. (* monad/proofs/misc.v *)
 Require Import bedrock.auto.invariants.
 Require Import bedrock.auto.cpp.proof.
 Require Import bedrock.auto.cpp.tactics4.
+
+Require Import monad.proofs.misc. (* monad/proofs/misc.v *)
 Require Import monad.proofs.demomisc.
 Require Import monad.proofs.demoprf.
 From AAC_tactics Require Import AAC.
@@ -20,109 +20,62 @@ Disable Notation drop.
 Disable Notation "`div`" (all).
 Disable Notation intR.
 Disable Notation uintR.
-Lemma lose_resources `{cpp_logic} (P:mpred): P |-- emp.
-Proof using.
-  go.
-Qed.
-
-Ltac lose_resources := try iStopProof; apply lose_resources.
 
 Import linearity.
-(** start recording *)
 
-(** [gcd_proof] *)
+
+(** start recording.
+Exercises:
+ *)
+
 Notation memory_order_seq_cst := 5.
 
 Section with_Sigma.
-  Context `{Sigma:cpp_logic} {CU: genv}.
+  Context `{Sigma:cpp_logic}  {CU: genv}.
   Context  {MODd : demo2.module ⊧ CU}.
-  Definition atomic_core_field_offset : offset. Proof. Admitted.
-  Definition atomicR (ty:type) (q : cQp.t) (v : val) : Rep :=
-    structR (Ninst "std::atomic" [Atype ty]) q
-    ** o_base CU (Ninst "std::atomic" [Atype ty]) (Ninst "std::__atomic_base" [Atype ty]) |-> structR  (Ninst "std::__atomic_base" [Atype ty]) q
-    ** atomic_core_field_offset |-> primR ty q v.
 
-(** Properties of [atomicR] *)
-Section atomicR.
-  Definition ns := (nroot .@@ "::SpinLock").
+    #[ignore_errors]
+    cpp.spec "std::__atomic_base<int>::exchange(int, enum std::memory_order)"  as int_exchange_spec with
+            (λ this : ptr,
+       \arg{(x : Z)} "v" (Vint x)
+       \arg "order" (Vint memory_order_seq_cst)
+       \let pd := this ,, o_derived CU "std::__atomic_base<int>" "std::atomic<int>"  
+       \pre{Q : Z → mpred}
+         AC1 << ∀ y : Z, pd |-> atomicR "int" (cQp.mut 1) (Vint y)>> @ ⊤, ∅
+            << pd |-> atomicR "int" (cQp.mut 1) (Vint x), COMM Q y >> 
+       \post{y : Z}[Vint y]
+       Q y).
 
-  #[global] Instance atomicR_frac T : CFracSplittable_1 (atomicR T).
-  Proof.  solve_cfrac. Qed.
-
-  #[global] Instance atomic_type_ptrR_observe ty v q
-    : Observe (type_ptrR (Tnamed (Ninst "std::atomic" [Atype ty]))) (atomicR ty v q) := _.
-
-  #[global] Instance atomic_type_ptrR_base_observe ty v q (p:ptr)
-    : Observe (type_ptr (Tnamed (Ninst "std::__atomic_base" [Atype ty])) (p,, o_base CU (Ninst "std::atomic" [Atype ty]) (Ninst "std::__atomic_base" [Atype ty]))) (p |-> atomicR ty v q).
-  Proof.
-    apply observe_intro;[exact _|].
-    iIntrosDestructs.
-    unfold atomicR.
-    hideRhs.
-    go.
-    unhideAllFromWork.
-    go.
-  Qed.
+    #[ignore_errors]
+    cpp.spec "std::__atomic_base<int>::load(enum std::memory_order) const"  as int_load_spec with
+            (λ this : ptr,
+       \let pd := this ,, o_derived CU "std::__atomic_base<int>" "std::atomic<int>"  
+       \arg "order" (Vint memory_order_seq_cst)
+       \pre{ (q:Qp) (InvOut : Z → mpred)}
+         AC1 << ∀ y : Z, pd |-> atomicR "int" q (Vint y)>> @ ⊤, ∅
+                      << pd |-> atomicR "int" q (Vint y), COMM InvOut y >> 
+       \post{y : Z}[Vint y]
+       InvOut y).
+    #[ignore_errors]
+    cpp.spec "std::atomic<bool>::exchange(bool, enum std::memory_order)"  as exchange_spec with
+            (λ this : ptr,
+       \arg{(x : bool)} "v" (Vbool x)
+       \arg "order" (Vint memory_order_seq_cst)
+       \pre{Q : bool → mpred}
+         AC1 << ∀ y : bool, this |-> atomicR Tbool (cQp.mut 1) (Vbool y)>> @ ⊤, ∅
+            << this |-> atomicR Tbool (cQp.mut 1) (Vbool x), COMM Q y >> 
+       \post{y : bool}[Vbool y]
+       Q y).
+    #[ignore_errors]
+    cpp.spec "std::atomic<bool>::store(bool, enum std::memory_order)"  as store_spec with
+(λ this : ptr,
+       \arg{(Q : mpred) (x : bool)} "v" (Vbool x)
+       \arg "memorder" (Vint 5)
+       \pre
+         AC1 << ∀ y : bool, this |-> atomicR Tbool (cQp.mut 1) (Vbool y)>> @ ⊤, ∅
+            << this |-> atomicR Tbool (cQp.mut 1) (Vbool x), COMM Q >> 
+                                                               \post    Q).
   
-  #[global] Instance atomic_agree ty v1 v2 q1 q2
-    : Observe2 [| v1 = v2 |] (atomicR ty q1 v1) (atomicR ty q2 v2) := _.
-
-  #[global] Instance atomic_agree_inj `{Vinj : A -> val} `{!Inj eq eq Vinj} ty v1 v2 q1 q2
-    : Observe2 [| v1 = v2 |] (atomicR ty q1 (Vinj v1)) (atomicR ty q2 (Vinj v2)).
-  Proof. exact: (observe2_inj Vinj). Qed.
-
-  Definition learn_atomic_val (p : ptr) ty v1 v2 q1 q2
-    : Learnable (p |-> atomicR ty q1 v1) (p |-> atomicR ty q2 v2) [v2=v1].
-  Proof. solve_learnable. Qed.
-
-  Definition learn_atomic_val_UNSAFE (p : ptr) ty v1 v2 q1 q2
-    : Learnable (p |-> atomicR ty q1 v1) (p |-> atomicR ty q2 v2) [v2=v1; q1=q2].
-  Proof. solve_learnable. Qed.
-  (** [atomicR ty q v] implies that value [v] has type [ty]. *)
-  Lemma atomicR_has_type_prop ty v q :
-    Observe [| has_type_prop v ty |] (atomicR ty q v).
-  Proof. refine _. Qed.
-End atomicR.
-
-Opaque atomicR.
-  Definition fwd_later_exist := [FWD] (@bi.later_exist).
-  Definition fwd_later_sep := [FWD] (@bi.later_sep).
-  Definition bwd_later_exist := [BWD_MW->] (@bi.later_exist).
-  Definition bwd_later_sep := [BWD_MW->] (@bi.later_sep).
-  Definition fwd_at_later := [FWD<-] (@_at_later).
-  Hint Resolve fwd_later_exist fwd_later_sep bwd_later_exist
-    bwd_later_sep : br_opacity.
-
-(* open all cinvq invariants then open rest. used in callAtomicCommitCinv*)
-Ltac openCinvqsRest :=
-  repeat openCinvq;
-  work using fwd_later_exist, fwd_later_sep;
-  repeat removeLater;
-  iApply fupd_mask_intro;[set_solver |]; (* openRest *)
-  iIntrosDestructs.
-
-(**
-   the RHS of your goal should look like a permutation of
-   [[
-   AC pre post ?Q ** (forall ..., ?Q ... -* ...)
-   ]]
-  it first calls [callAtomicCommit] to instantiate the public post Q.
-  then it opens all cinvq invariants
-  then it opens everything else (change the goal from [|={⊤ \ ..\ ... ,∅}=> U)] to  [|={∅}=> U)])
-  and then "does iModIntro" so that you can start proving U which is typically of the form [pre ** ...]
- *)
-Ltac callAtomicCommitCinv :=
-  repeat (iExists _);
-  callAtomicCommit;
-  openCinvqsRest.
-
-(* applies to goals that look like [|-- AC pre post Q] or [|-- AU pre post Q]  in IPM: only 1 conjuct in conclusion and not 2, where [callAtomicCommitCinv] works. it sets up the proof of AC/AU by doing the usual initialization
- and opening all invariants and rest so that you can immediately begin proving [pre] *)
-Ltac proveAuAc :=
-  (iAcIntro || iAuIntro);
-  (unfold commit_acc || unfold atomic_acc);
-  openCinvqsRest.
-
 (*
 Hint Resolve learn_atomic_val : br_opacity.
 *)  
@@ -157,24 +110,6 @@ Hint Resolve learn_atomic_val : br_opacity.
   cpp.spec "gcdl(unsigned int*, unsigned int)" as gcdl_spec with (gcdl_spec_core).
   cpp.spec "parallel_gcdl(unsigned int*, unsigned int)" as parallel_gcdl_spec with (gcdl_spec_core).
 
-  Compute (findBodyOfFnNamed2 module (isFunctionNamed2 "fold_left")).
-
-  #[ignore_errors]
-  cpp.spec "fold_left(unsigned int*, unsigned int, unsigned int(*)(unsigned int,unsigned int), unsigned int)" as fold_left_spec with (
-      \arg{numsp:ptr} "nums" (Vptr numsp)
-      \prepost{(l: list Z) (q:Qp)} numsp |-> arrayR uint (fun i:Z => primR uint q i) l
-      \arg "size" (Vint (length l))
-      \arg{fptr} "f" (Vptr fptr)
-      \arg{initv} "init" (Vint initv)
-      \pre{fm: Z->Z->Z} fptr |-> cpp_specR (tFunction "unsigned int" ["unsigned int*"%cpp_type; "unsigned int"%cpp_type])
-      (
-        \arg{av:Z} "a" (Vint av)
-        \arg{bv:Z} "b" (Vint bv)
-        \post [Vint (fm av bv)] emp
-       )
-      \post [Vint (fold_left fm l initv)] emp).
-
-    
   (** * 2+ ways to split an arrays *)
   (** split fraction: both threads can read entire array *)
   Lemma fractionalSplitArrayR (numsp:ptr) (l: list Z) (q:Qp):
@@ -201,13 +136,227 @@ Hint Resolve learn_atomic_val : br_opacity.
     rewrite arrayR_split; eauto. go. 
   Qed.
 
-  (** Structs: Point2D *)
+
+  (** *Parallelizing a sequence of operations
+
+(((i o a1) o a2 ) o a3 )        (((i o a4) o a5 ) o a6 )
+                    \               /
+                     \             /
+                      \           /
+                   left_result   right_result
+                          \       /
+                           \     /
+                            \   /
+                        (left_result o right_result)
+
+*)
+
+  Hint Rewrite @fold_left_app: syntactic.
+  Existing Instance UNSAFE_read_prim_cancel.
+  
+  Lemma gcd_proof: denoteModule module |-- gcd_spec.
+  Proof using.
+    rewrite <- demoprf.gcd_proof.
+    apply denoteModule_weaken.
+    apply module_le_true.
+    exact _.
+  Qed.
+  
+  Lemma gcdl_proof: denoteModule module |-- gcdl_spec.
+  Proof using MODd with (fold cQpc).
+    verify_spec.
+    slauto.
+    wp_for (fun _ => Exists iv:nat,
+        i_addr |-> primR uint 1 iv
+        ** [| iv <= length l |]%nat
+        ** result_addr |-> primR uint 1 ((fold_left Z.gcd (firstn iv l) 0))).
+    go. iExists 0%nat. go.
+    wp_if.
+    {
+      slauto.
+      eapplyToSomeHyp @arrayR_cell2.
+      forward_reason.
+      rewrite -> autogenhypr.
+      hideRhs.
+      go.
+      unhideAllFromWork.
+      slauto. (* call to gcd. we have already proved it's spec *)
+      wapply gcd_proof. work. (* gcd_spec is now in context *)
+      go. (* loop body finished, reistablish loopinv *)
+      iExists (1+iv)%nat.
+      slauto.
+      simpl.
+      go.
+      rewrite -> autogenhypr.
+      go.
+    }
+    {
+      slauto.
+      assert (iv=length l) as Heq by lia.
+      subst.
+      autorewrite with syntactic.
+      go.
+    }
+  Qed.
+
+  
+      Compute (Z.quot (-5) 4).
+      Compute (Z.div (-5) 4).
+      Set Default Goal Selector "!".
+  cpp.spec (Nscoped 
+              "parallel_gcdl(unsigned int*, unsigned int)::@0" Ndtor)  as lam2destr  inline.
+
+
+  Lemma pgcdl_proof: denoteModule module
+                       ** (thread_class_specs "parallel_gcdl(unsigned int*, unsigned int)::@0")
+                       |-- parallel_gcdl_spec.
+  Proof using MODd with (fold cQpc).
+    unfold thread_class_specs.
+    verify_spec'.
+    wapply gcdl_proof.
+    wapply gcd_proof. go.
+    name_locals.
+    wapplyObserve  obsUintArrayR.
+    eagerUnifyU. work.
+    aggregateRepPieces gcdlLambda_addr.
+    go.
+    hideP ps.
+    Opaque Nat.div.
+    assert ( (length l/ 2 <= length l)%nat) as Hle.
+    {
+      rewrite <- Nat.div2_div.
+      apply Nat.le_div2_diag_l.
+    }
+    nat2ZNLdup.
+    rewrite (primr_split nums_addr).
+    rewrite (primr_split mid_addr).
+    simpl in *.
+    closed.norm closed.numeric_types.
+    rewrite -> arrayR_split with (i:=((length l)/2)%nat) (xs:=l) by lia;
+      go... (* array ownership spit into 2 pieces *)
+    revertAdrs constr:([numsp; resultl_addr; nums_addr; mid_addr]).
+    repeat rewrite bi.wand_curry.
+    intantiateWand.
+    instWithPEvar taskPost.
+    go.
+    iSplitL "".
+    { verify_spec'.
+      go.
+      iExists _. eagerUnifyU.
+      autorewrite with syntactic. go.
+      erefl.
+    }
+    unhideAllFromWork.
+    autorewrite with syntactic. go. 
+    iExists _. eagerUnifyU. 
+    autorewrite with syntactic. go.
+    wapply @arrayR_combinep. eagerUnifyU.
+    autorewrite with syntactic. go.
+    (* c++ semantics computes ... postcond requires *)
+    icancel (cancel_at p);[| go].
+    do 2 f_equiv.
+    symmetry.
+    apply fold_split_gcd.
+    auto.
+  Qed.
+  
+  Lemma fold_split_gcd  (l: list Z) (pl: forall a, In a l -> 0 <= a) (lSplitSize: nat):
+    fold_left Z.gcd l 0=
+      Z.gcd (fold_left Z.gcd (firstn lSplitSize l) 0) (fold_left Z.gcd (skipn lSplitSize l) 0).
+  Proof using. apply misc.fold_split_gcd; auto. Qed.
+
+  Lemma fold_split {A:Type} (f: A->A->A)(asoc: Associative (=) f)
+    (id: A) (lid: LeftId (=) id f) (rid: RightId (=) id f) (l: list A) (lSplitSize: nat):
+    fold_left f l id =
+      f (fold_left f (firstn lSplitSize l) id)
+        (fold_left f (skipn  lSplitSize l) id).
+  Proof.
+    rewrite <- (take_drop lSplitSize) at 1.
+    rewrite fold_left_app.
+    rewrite fold_id2.
+    aac_reflexivity.
+  Qed.
+
+  #[ignore_errors]
+  cpp.spec "fold_left(unsigned int*, unsigned int, unsigned int(*)(unsigned int,unsigned int), unsigned int)" as fold_left_spec with (
+      \arg{numsp:ptr} "nums" (Vptr numsp)
+      \prepost{(l: list Z) (q:Qp)} numsp |-> arrayR uint (fun i:Z => primR uint q i) l
+      \arg "size" (Vint (length l))
+      \arg{fptr} "f" (Vptr fptr)
+      \arg{initv} "init" (Vint initv)
+      \pre{fm: Z->Z->Z} fptr |->
+          cpp_specR (tFunction "unsigned int" ["unsigned int"%cpp_type; "unsigned int"%cpp_type])
+            (
+              \arg{av:Z} "a" (Vint av)
+                \arg{bv:Z} "b" (Vint bv)
+                \post [Vint (fm av bv)] emp
+            )
+      \post [Vint (fold_left fm l initv)] emp).
+
+  #[ignore_errors]
+  cpp.spec "fold_left_parallel(unsigned int*, unsigned int, unsigned int(*)(unsigned int,unsigned int), unsigned int)" as fold_left_spec with (
+      \arg{numsp:ptr} "nums" (Vptr numsp)
+      \prepost{(l: list Z) (q:Qp)} numsp |-> arrayR uint (fun i:Z => primR uint q i) l
+      \arg "size" (Vint (length l))
+      \arg{fptr} "f" (Vptr fptr)
+      \pre{fm: Z->Z->Z} fptr |->
+          cpp_specR (tFunction "unsigned int" ["unsigned int"%cpp_type; "unsigned int"%cpp_type])
+            (
+              \arg{av:Z} "a" (Vint av)
+                \arg{bv:Z} "b" (Vint bv)
+                \post [Vint (fm av bv)] emp
+            )
+      \pre [| Associative (=) fm |]
+      \arg{initv} "init" (Vint initv)
+      \pre [| LeftId (=) initv fm |]
+      \pre [| RightId (=) initv fm |]
+      \post [Vint (fold_left fm l initv)] emp).
+  
+  Lemma fold_left_prf : denoteModule module |-- fold_left_spec.
+  Proof using MODd.
+    verify_spec'.
+    slauto.
+    wp_for (fun _ => Exists iv:nat,
+        i_addr |-> primR uint 1 iv
+        ** [| iv <= length l |]%nat
+        ** result_addr |-> primR uint 1 ((fold_left fm (firstn iv l) initv))).
+    unfold cQpc.
+    go.
+    Set Printing Coercions.
+    rewrite <- (bi.exist_intro 0%nat).
+    go.
+    wp_if.
+    {
+      slauto.
+      Set Printing Implicit.
+      eapplyToSomeHyp @arrayR_cell2.
+      forward_reason.
+      rewrite -> autogenhypr.
+      hideRhs.
+      go.
+      unhideAllFromWork.
+      slauto. (* loop body finished, reistablish loopinv *)
+      iExists (1+iv)%nat.
+      slauto.
+      rewrite -> autogenhypr.
+      go.
+    }
+    {
+      slauto.
+      assert (iv=length l) as Heq by lia.
+      subst.
+      autorewrite with syntactic.
+      go.
+    }
+  Qed.
+  
+  (** Structs: Node [c] *)
   Definition NodeR `{Σ : cpp_logic, σ : genv} (q: cQp.t) (data: Z) (nextLoc: ptr): Rep :=
     structR "Node" q
     ** _field "Node::data_" |-> primR Ti32                       (cQp.mut q) data
     ** _field "Node::next_" |-> primR (Tptr (Tnamed "Node")) (cQp.mut q) (Vptr nextLoc).
 
-  (** Structs: LinkedList *)
+  (** Structs: LinkedList [c] *)
 
 
   Fixpoint ListR (q : cQp.t) (l : list Z) : Rep :=
@@ -215,7 +364,6 @@ Hint Resolve learn_atomic_val : br_opacity.
     | [] => nullR
     | hd :: tl => Exists (p : ptr), NodeR q hd p ** pureR (p |-> ListR q tl)
     end.
-
 
   Example listRUnfold (q:Qp) (head:ptr): head |-> ListR 1 [4;5;6] |--
     Exists node5loc node6loc,
@@ -280,36 +428,8 @@ Hint Resolve learn_atomic_val : br_opacity.
      \pre{l} lp |-> ListR 1 l
      \post{r}[Vptr r] Exists ls, r |-> ListR (1) ls ** [| sorted ls /\ l ≡ₚ ls|]).
 
-  Lemma fold_id {A:Type} (f: A->A->A) (asoc: Associative (=) f)
-    (start id: A) (lid: LeftId (=) id f) (rid: RightId (=) id f) (l: list A):
-    fold_left f l start = f start (fold_left f l id).
-  Proof using.
-    hnf in lid.
-    hnf in rid.
-    revert start.
-    induction l; auto.
-    simpl.
-    simpl. rewrite lid.
-    intros.
-    simpl.
-    rewrite IHl.
-    symmetry.
-    rewrite IHl.
-    aac_reflexivity.
-  Qed.
 
-  Lemma fold_split {A:Type} (f: A->A->A)(asoc: Associative (=) f)
-    (id: A) (lid: LeftId (=) id f) (rid: RightId (=) id f) (l: list A) (lSplitSize: nat):
-    fold_left f l id =
-      f (fold_left f (firstn lSplitSize l) id)
-        (fold_left f (skipn  lSplitSize l) id).
-  Proof.
-    rewrite <- (take_drop lSplitSize) at 1.
-    rewrite fold_left_app.
-    rewrite fold_id.
-    aac_reflexivity.
-  Qed.
-  
+
   (** Passing resources between running threads
 
 last session, we saw:
@@ -348,112 +468,35 @@ Parent: Child.join
 (** *Concurrent Invariants 
 [c200,345]
    *)
-
-  Notation inv := (cinvq (nroot .@@ "::demo2")).
   
-Lemma cinvq_alloc `{Σ : cpp_logic} (E : coPset) (N : namespace) (P : mpred) :
-  WeaklyObjective P → ▷ P |-- |={E}=> ∃ γ : gname, cinvq N γ 1 P.
-Proof.
-  intros.
-  unfold cinvq.
-  wapply (cinv_alloc E N P).
-  work.
-  iModIntro.
-  ework.
-  eagerUnifyU. go.
-Qed.
 
-Lemma cinvq_alloc_no_shared_pages `{Σ : cpp_logic} (E : coPset) (N : namespace) (P : mpred) :
-  ▷ P |-- |={E}=> ∃ γ : gname, cinvq N γ 1 P.
-  Proof.
-    intros.
-    apply cinvq_alloc.
-  Admitted.
+Example boxedResource (P:mpred) (invId: gname): mpred := cinv invId 1 P.
 
-Example boxedResource (P:mpred) (invId: gname): mpred := inv invId 1 P.
-
-Lemma mut_mut_add: ∀ q1 q2 : Qp, cQp.mut (q1 + q2) = (cQp.mut q1 + cQp.mut q2)%cQp.
-Proof. intros. reflexivity. Qed.
-  Ltac solveCqpeq :=
-    repeat match goal with
-        H:Qp |- _ => destruct H; simpl in *
-      end;
-      unfold cQpc, cQp.scale; simpl in *;
-      repeat rewrite <- mut_mut_add;
-       f_equal;              
-        solveQpeq;
-        solveQeq.
-
-Lemma splitcinvq (P:mpred) ns (invId: gname) (q:Qp):
-  cinvq ns invId q P |-- cinvq ns invId (q/2) P ** cinvq ns invId (q/2) P.
-Proof using.
-  rewrite <- (@fractional _ _ (cinvq_frac _)).
-  f_equiv.
-  solveCqpeq.
-Qed.
   
 Lemma splitInv (P:mpred) (invId: gname) (q:Qp):
-  inv invId q P |-- inv invId (q/2) P ** inv invId (q/2) P.
+  cinv invId q P |-- cinv invId (q/2) P ** cinv invId (q/2) P.
 Proof using.
   apply splitcinvq.
 Qed.
 
   cpp.spec "bar()" as bar_spec with (
-      \prepost{q invId} inv q invId (∃ zv, _global "z" |-> primR "int" 1 zv)
+      \prepost{q invId} cinv q invId (∃ zv, _global "z" |-> primR "int" 1 zv)
       \post emp
     ).
   Lemma bar_prf : denoteModule module |-- bar_spec.
   Proof using.
     verify_spec.
     go.
-  Abort. (* highlight. not an atomic op. cannot open the inv box *)
+  Abort. (* highlight. not an atomic op. cannot open the cinv box *)
 
   cpp.spec "setU(int)" as setU_spec with (
-      \prepost{q invId} inv q invId (∃ zv:Z, _global "u" |-> atomicR "int" 1 zv)
+      \prepost{q invId} cinv q invId (∃ zv:Z, _global "u" |-> atomicR "int" 1 zv)
       \arg{value} "value" (Vint value)
       \post emp
       ).
-  
-    #[ignore_errors]
-    cpp.spec "std::__atomic_base<int>::exchange(int, enum std::memory_order)"  as int_exchange_spec with
-            (λ this : ptr,
-       \arg{(x : Z)} "v" (Vint x)
-       \arg "order" (Vint memory_order_seq_cst)
-       \let pd := this ,, o_derived CU "std::__atomic_base<int>" "std::atomic<int>"  
-       \pre{Q : Z → mpred}
-         AC1 << ∀ y : Z, pd |-> atomicR "int" (cQp.mut 1) (Vint y)>> @ ⊤, ∅
-            << pd |-> atomicR "int" (cQp.mut 1) (Vint x), COMM Q y >> 
-       \post{y : Z}[Vint y]
-       Q y).
-
+      
     Opaque coPset_difference.
-    Lemma peek_cinvq a b c P (C:mpred) learn:
-      ▷ P |-- bupd (▷ P ** learn) 
-      -> (learn -* cinvq a b c P -*  |={⊤}=> C) |-- cinvq a b c P -*  |={⊤}=> C.
-    Proof using.
-      intros hl.
-      go.
-      openCinvq.
-      rewrite hl.
-      ghost.
-      go.
-      wapply invariants.close_cinvQR4.
-      eagerUnifyU.
-      unhideAllFromWork.
-      go.
-      iModIntro.
-      iFrame.
-    Qed.
-
-    Lemma admitReferenceTo ty ptr : emp |-- reference_to ty ptr.
-    Proof. Admitted.
-    Ltac solveRefereceTo :=
-      IPM.perm_right ltac:(fun R _ =>
-                             match R with
-                             | reference_to ?ty ?p =>
-                                 wapply (admitReferenceTo ty p)
-                             end
-                          ).
+    Opaque atomicR.
 Ltac slauto := (slautot ltac:(autorewrite with syntactic; try solveRefereceTo)); try iPureIntro.
   Lemma setU_prf: denoteModule module ** int_exchange_spec |-- setU_spec.
   Proof using MODd.
@@ -470,18 +513,8 @@ Ltac slauto := (slautot ltac:(autorewrite with syntactic; try solveRefereceTo));
     go.
   Qed.
     
-    #[ignore_errors]
-    cpp.spec "std::__atomic_base<int>::load(enum std::memory_order) const"  as int_load_spec with
-            (λ this : ptr,
-       \let pd := this ,, o_derived CU "std::__atomic_base<int>" "std::atomic<int>"  
-       \arg "order" (Vint memory_order_seq_cst)
-       \pre{ (q:Qp) (InvOut : Z → mpred)}
-         AC1 << ∀ y : Z, pd |-> atomicR "int" q (Vint y)>> @ ⊤, ∅
-                      << pd |-> atomicR "int" q (Vint y), COMM InvOut y >> 
-       \post{y : Z}[Vint y]
-       InvOut y).
   cpp.spec "setThenGetU(int)" as setGetU_spec_wrong with (
-      \prepost{q invId} inv q invId (∃ zv:Z, _global "u" |-> atomicR "int" 1 zv)
+      \prepost{q invId} cinv q invId (∃ zv:Z, _global "u" |-> atomicR "int" 1 zv)
       \arg{value} "value" (Vint value)
       \post [Vint value] emp
         ).
@@ -508,7 +541,7 @@ Ltac slauto := (slautot ltac:(autorewrite with syntactic; try solveRefereceTo));
   Abort.
 
   cpp.spec "setThenGetU(int)" as setGetU_spec with (
-      \prepost{q invId} inv q invId (∃ zv:Z, _global "u" |-> atomicR "int" 1 zv)
+      \prepost{q invId} cinv q invId (∃ zv:Z, _global "u" |-> atomicR "int" 1 zv)
       \arg{value} "value" (Vint value)
       \post{any:Z} [Vint any] emp
       ).
@@ -532,7 +565,7 @@ Ltac slauto := (slautot ltac:(autorewrite with syntactic; try solveRefereceTo));
   Qed.
 
   cpp.spec "setThenGetU(int)" as setGetU_spec2 with (
-      \prepost{q invId} inv q invId (∃ zv:Z, _global "u" |-> atomicR "int" 1 zv ** [| isPrime zv |])
+      \prepost{q invId} cinv q invId (∃ zv:Z, _global "u" |-> atomicR "int" 1 zv ** [| isPrime zv |])
       \arg{value} "value" (Vint value)
       \post{any:Z} [Vint any] emp
       ).
@@ -548,7 +581,7 @@ Ltac slauto := (slautot ltac:(autorewrite with syntactic; try solveRefereceTo));
     go. 
   Abort.
   cpp.spec "setThenGetU(int)" as setGetU_spec_prime with (
-      \prepost{q invId} inv q invId (∃ zv:Z, _global "u" |-> atomicR "int" 1 zv ** [| isPrime zv |])
+      \prepost{q invId} cinv q invId (∃ zv:Z, _global "u" |-> atomicR "int" 1 zv ** [| isPrime zv |])
       \arg{value} "value" (Vint value)
       \pre [| isPrime value |] 
       \post{any:Z} [Vint any] [| isPrime value |]
@@ -587,13 +620,14 @@ next .. examples of more interesting loopinv
   (** * BlockState analog: *)
 
   Definition ucinv (q:Qp) (invId: gname): mpred
-    := inv invId q (∃ zv:Z, _global "u" |-> atomicR "int" (1/2) zv ** [| isPrime zv |]).
-  (** only half in inv *)
-  
+    := cinv invId q (∃ zv:Z, _global "u" |-> atomicR "int" (1/2) zv ** [| isPrime zv |]).
+  (** only half in cinv *)
+
+
   Definition uAuthR (invId: gname) (uv: Z): mpred
     := ucinv (1/2) invId ** _global "u" |-> atomicR "int" (1/2) uv.
 
-  (* no fraction argument in uAuthR
+  (* no fraction argument in uAuthR:
      p1: ucinv (1/4) invId ** _global "u" |-> atomicR "int" (1/4) uv.
 
      p2: ucinv (1/4) invId ** _global "u" |-> atomicR "int" (1/4) uv.
@@ -602,20 +636,8 @@ next .. examples of more interesting loopinv
   Definition uFragR (q:Qp) (invId: gname) : mpred := ucinv (q/2) invId.
   (* different from fractional ownership: [_global "u" |-> atomicR "int" q 3], [_global "x" |-> primR "int" q 3] *)
 
-  Lemma atomicr_split (p:ptr) ty (q:Qp) v :
-    p|-> atomicR ty (cQp.mut q) v -|- (p |-> atomicR ty (cQp.mut q/2) v) ** p |-> atomicR ty (cQp.mut q/2) v.
-  Proof using.
-    rewrite -> cfractional_split_half with (R := fun q => atomicR ty q v);[| exact _].
-    rewrite _at_sep.
-    f_equiv; f_equiv; f_equiv;
-      solveCqpeq.
-  Qed.
-  Definition atomicrC := [CANCEL] atomicr_split.
   Hint Resolve atomicrC : br_opacity.
-  Definition lcinvqg_unsafe a1 g1 q1 P1 a2 g2 q2 P2:
-    Learnable (cinvq a1 g1 q1 P1) (cinvq a2 g2 q2 P2) [g1=g2] := ltac:(solve_learnable).
   Existing Instance lcinvqg_unsafe.
-  Definition cinvqC := [CANCEL] splitcinvq.
   Hint Resolve cinvqC : br_opacity.
   Lemma init (initv:Z) E:
     _global "u" |-> atomicR "int" 1 initv ** [| isPrime initv |]
@@ -642,6 +664,11 @@ next .. examples of more interesting loopinv
       \post{any:Z} [Vint any] [| isPrime any|]
       ).
   
+  cpp.spec "getU()" as getU_spec_auth with (
+      \prepost{invId uval} uAuthR invId uval
+      \post{any:Z} [Vint uval] [| isPrime uval|]
+      ).
+  
   cpp.spec "setThenGetU(int)" as setThenGet_spec2 with (
       \pre{(oldvalue:Z) invId} uAuthR invId oldvalue
       \arg{newvalue:Z} "value" (Vint newvalue)
@@ -649,66 +676,6 @@ next .. examples of more interesting loopinv
       \post [Vint newvalue] uAuthR invId newvalue
       ).
 
-    Lemma observe_elim_rep (Q P : Rep) (p:ptr): Observe Q P → p |-> P ⊢ p|->(P ∗ Q).
-    Proof using.
-      intros Ho.
-      apply _at_mono.
-      wapplyObserve Ho.
-      go.
-    Qed.
-    
-    Search Observe Rep.
-        
-  Lemma observe_2_elim_rep Q P1 P2 (p:ptr) {O : Observe2 Q P1 P2} : p|->P1 ⊢ p|-> P2 -∗ p|->P1 ∗ p|->P2 ∗ p|->Q.
-  Proof.
-    iIntros. iStopProof.
-    repeat rewrite <- _at_sep.
-    apply _at_mono.
-    wapplyObserve O.
-    go.
-  Qed.
-
-Ltac wapplyObserveRep lemma:=
-  try intros;
-  idtac;
-  [
-    wapply (@observe_elim_rep _ _ _ (lemma)) || wapply (@observe_elim_rep _ _ _ (lemma _))
-    || wapply (@observe_elim_rep _ _ _ (lemma _ _)) || wapply (@observe_elim_rep _ _ _ (lemma _ _ _))
-    || wapply (@observe_elim_rep _ _ _ (lemma _ _ _ _)) || wapply (@observe_elim_rep _ _ _ (lemma _ _ _ _ _))
-    || wapply (@observe_elim_rep _ _ _ (lemma _ _ _ _ _ _)) || wapply (@observe_elim_rep _ _ _ (lemma _ _ _ _ _ _ _))
-    || wapply (@observe_elim_rep _ _ _ (lemma _ _ _ _ _ _ _ _)) || wapply (@observe_elim_rep _ _ _ (lemma _ _ _ _ _ _ _ _ _))
-    || wapply (@observe_elim_rep _ _ _ (lemma _ _ _ _ _ _ _ _ _ _)) || wapply (@observe_elim_rep _ _ _ (lemma _ _ _ _ _ _ _ _ _ _ _))
-    
-    || wapply (@observe_2_elim_rep _ _ _ _ (lemma)) || wapply (@observe_2_elim_rep _ _ _ _ (lemma _))
-    || wapply (@observe_2_elim_rep _ _ _ _ (lemma _ _)) || wapply (@observe_2_elim_rep _ _ _ _ (lemma _ _ _))
-    || wapply (@observe_2_elim_rep _ _ _ _ (lemma _ _ _ _)) || wapply (@observe_2_elim_rep _ _ _ _ (lemma _ _ _ _ _))
-    || wapply (@observe_2_elim_rep _ _ _ _ (lemma _ _ _ _ _ _)) || wapply (@observe_2_elim_rep _ _ _ _ (lemma _ _ _ _ _ _ _))
-    || wapply (@observe_2_elim_rep _ _ _ _ (lemma _ _ _ _ _ _ _ _)) || wapply (@observe_2_elim_rep _ _ _ _ (lemma _ _ _ _ _ _ _ _ _))
-    || wapply (@observe_2_elim_rep _ _ _ _ (lemma _ _ _ _ _ _ _ _ _ _)) || wapply (@observe_2_elim_rep _ _ _ _ (lemma _ _ _ _ _ _ _ _ _ _ _))
-    
-  ].
-    Lemma atomicR_combine (p:ptr) (q1 q2: Qp) (v1 v2 : val) ty:
-    p |-> atomicR ty q1 v1 ** p |-> atomicR ty q2 v2
-      |-- p |-> atomicR ty (q1+q2) v1 ** [| v1 = v2 |].
-    Proof using.
-      go.
-      wapplyObserveRep atomic_agree. eagerUnifyU. go.
-      rewrite -> @cfractional.cfractional with (P := fun q => atomicR ty q v1);[| exact _].
-      go.
-    Qed.
-    Lemma atomicR_combine_half (p:ptr) (q: Qp) (v1 v2 : val) ty:
-    p |-> atomicR ty (q/2) v1 ** p |-> atomicR ty (q/2) v2
-      |-- p |-> atomicR ty q v1 ** [| v1 = v2 |].
-    Proof using.
-      rewrite atomicR_combine.
-      go.
-      iClear "#".
-      iStopProof.
-      apply _at_mono.
-      f_equiv.
-      solveCqpeq.
-    Qed.
-    Definition atomicR_combineF := [FWD] atomicR_combine.
   
   Lemma setGetU_prf2: denoteModule module ** int_exchange_spec  ** int_load_spec |-- setThenGet_spec2.
   Proof using MODd with (fold cQpc).
@@ -724,7 +691,7 @@ Ltac wapplyObserveRep lemma:=
     iModIntro.
     (** closed the invariant and se still have 1/2 left [g11,12].
         crucial when we call load next: [g11,12]
-        other threads can race but they can only read. I own 1/2 of atomicR. other threads can only access the 1/2 in the inv *)
+        other threads can race but they can only read. I own 1/2 of atomicR. other threads can only access the 1/2 in the cinv *)
     go.
     callAtomicCommitCinv...
     (* had before [g11,12]. opening the invariant got this part [g] says u has value a and is IsPrime [g].
@@ -744,323 +711,18 @@ Ltac wapplyObserveRep lemma:=
   Qed.
     
   
-  Definition AWrapperR  (q: Qp) (invId: gname): Rep :=
-    structR "AWRapper" q **
-    as_Rep (fun this:ptr =>
-      inv invId q (∃ i:Z, this ,, _field "v" |-> atomicR "int" 1 i)).
-
-  (** above, i is ∃ quantified *)
-  Definition AWrapperRs  (q: Qp) (i:Z): Rep :=
-    structR "AWRapper" q **
-      _field "v" |-> atomicR "int" q (Vint i).
-
-  
-  cpp.spec "AWrapper::setValue(int)" as setValue_spec with (fun (this:ptr) =>
-     \prepost{q invid} this |-> AWrapperR q invid
-     \arg{newval:Z} "value" (Vint newval)
-     \post emp).
-  
-  cpp.spec "AWrapper::setValue(int)" as setValue_nonconcurrent_spec with (fun (this:ptr) =>
-     \pre{oldVal} this |-> AWrapperRs 1 oldVal
-     \arg{i:Z} "value" (Vint i)
-     \post this |-> AWrapperRs 1 i). (** but.. no other thread can call any method during this call *)
-
-  cpp.spec "AWrapper::getValue()" as getValue_spec with (fun (this:ptr) =>
-     \prepost{q invid} this |-> AWrapperR q invid
-     \post{any:Z} [Vint any] emp).
-
-  cpp.spec "AWrapper::getValue()" as getValue_nonconcurrent_spec with (fun (this:ptr) =>
-     \prepost{q (val:Z)} this |-> AWrapperRs q val
-     \post [Vint val] emp).
 
   Lemma as_Rep_meaning (f: ptr -> mpred) (base:ptr) :
     (base |-> as_Rep f)  -|- f base.
   Proof using. iSplit; go. Qed.
   
-  Definition AWrapperR2  (q: Qp) (invId: gname): Rep :=
-    structR "AWRapper" q **
-    as_Rep (fun this:ptr =>
-       inv invId q (∃ i:Z, this ,, _field "v" |-> atomicR "int" 1 i
-                        ** [| isPrime i |] )).
 
-  cpp.spec "AWrapper::setValue(int)" as setValue2_spec with (fun (this:ptr) =>
-     \prepost{q invId} this |-> AWrapperR2 q invId
-     \arg{i:Z} "value" (Vint i)
-     \pre [| isPrime i |] 
-     \post emp).
-
-  cpp.spec "AWrapper::getValue()" as getValue2_spec with (fun (this:ptr) =>
-     \prepost{q invid} this |-> AWrapperR2 q invid
-     \post{any:Z} [Vint any] [| isPrime any |]).
-
-  Opaque atomicR.
   Lemma duplPrime (i:Z) (this:ptr) :
     let p := this ,, _field "v" |-> atomicR "int" 1 i ** [| isPrime i |] in
     p |-- p ** [| isPrime i |].
   Proof using. go. Qed.
 
-  
-  
-  (** *Parallelizing a sequence of operations
-- e.g. sequence of operations monad transactions.
-- Commutativivity enables ||: a o b = b o a
-
-o commutative, with i as its left identity (forall x, i o x = x)
-
-fold_left o [a1;a2;a3;a4;a5;a6] i =
-((((((i o a1) o a2) o a3) o a4) o a5) o a6)
-
-
-(((i o a1) o a2 ) o a3 )        (((i o a4) o a5 ) o a6 )
-                    \               /
-                     \             /
-                      \           /
-                   left_result   right_result
-                          \       /
-                           \     /
-                            \   /
-                        (left_result o right_result)
-
-also, arrays
-*)
-
-  Hint Rewrite @fold_left_app: syntactic.
-  Existing Instance UNSAFE_read_prim_cancel.
-  
-  Lemma gcd_proof: denoteModule module |-- gcd_spec.
-  Proof using.
-    rewrite <- demoprf.gcd_proof.
-    apply denoteModule_weaken.
-    apply module_le_true.
-    exact _.
-  Qed.
-  
-  Lemma gcdl_proof: denoteModule module |-- gcdl_spec.
-  Proof using MODd with (fold cQpc).
-    verify_spec.
-    slauto.
-    wp_for (fun _ => Exists iv:nat,
-        i_addr |-> primR uint 1 iv
-        ** [| iv <= length l |]%nat
-        ** result_addr |-> primR uint 1 ((fold_left Z.gcd (firstn iv l) 0))).
-    go. iExists 0%nat. go.
-    wp_if.
-    {
-      slauto.
-      eapplyToSomeHyp @arrayR_cell2.
-      forward_reason.
-      rewrite -> autogenhypr.
-      hideRhs.
-      go.
-      unhideAllFromWork.
-      slauto. (* call to gcd. we have already proved it's spec *)
-      wapply gcd_proof. work. (* gcd_spec is now in context *)
-      go. (* loop body finished, reistablish loopinv *)
-      iExists (1+iv)%nat.
-      slauto.
-      simpl.
-      go.
-      rewrite -> autogenhypr.
-      go.
-    }
-    {
-      slauto.
-      assert (iv=length l) as Heq by lia.
-      subst.
-      autorewrite with syntactic.
-      go.
-    }
-  Qed.
-
-  Lemma fold_left_prf : denoteModule module |-- fold_left_spec.
-  Proof using.
-    verify_spec'.
-    slauto.
-    wp_for (fun _ => Exists iv:nat,
-        i_addr |-> primR uint 1 iv
-        ** [| iv <= length l |]%nat
-        ** result_addr |-> primR uint 1 ((fold_left fm (firstn iv l) initv))).
-    unfold cQpc.
-    go.
-    rewrite <- (bi.exist_intro 0%nat).
-    go.
-    wp_if.
-    {
-      slauto.
-      Set Printing Implicit.
-      eapplyToSomeHyp @arrayR_cell2.
-      forward_reason.
-      rewrite -> autogenhypr.
-      hideRhs.
-      go.
-      unhideAllFromWork.
-      slauto.
-      Hint Resolve @find_spec.find_cpp_specR : br_opacity.
-      go.
-      (*
-      wapply gcd_proof. work. (* gcd_spec is now in context *)
-      go. (* loop body finished, reistablish loopinv *)
-      iExists (1+iv)%nat.
-      slauto.
-      simpl.
-      go.
-      rewrite -> autogenhypr.
-      go.
-    }
-    {
-      slauto.
-      assert (iv=length l) as Heq by lia.
-      subst.
-      autorewrite with syntactic.
-      go.
-    } *)
-  Abort.
-  
-      Compute (Z.quot (-5) 4).
-      Compute (Z.div (-5) 4).
-      Set Default Goal Selector "!".
-  cpp.spec (Nscoped 
-              "parallel_gcdl(unsigned int*, unsigned int)::@0" Ndtor)  as lam2destr  inline.
-
-
-  Lemma pgcdl_proof: denoteModule module
-                       ** (thread_class_specs "parallel_gcdl(unsigned int*, unsigned int)::@0")
-                       |-- parallel_gcdl_spec.
-  Proof using MODd with (fold cQpc).
-    unfold thread_class_specs.
-    verify_spec'.
-    wapply gcdl_proof.
-    wapply gcd_proof. go.
-    name_locals.
-    wapplyObserve  obsUintArrayR.
-    eagerUnifyU. work.
-    aggregateRepPieces gcdlLambda_addr.
-    go.
-    hideP ps.
-    Opaque Nat.div.
-    assert ( (length l/ 2 <= length l)%nat) as Hle.
-    {
-      rewrite <- Nat.div2_div.
-      apply Nat.le_div2_diag_l.
-    }
-    nat2ZNLdup.
-    rewrite (primr_split nums_addr).
-    rewrite (primr_split mid_addr).
-    simpl in *.
-    closed.norm closed.numeric_types.
-    rewrite -> arrayR_split with (i:=((length l)/2)%nat) (xs:=l) by lia;
-      go... (* array ownership spit into 2 pieces *)
-    revertAdrs constr:([numsp; resultl_addr; nums_addr; mid_addr]).
-    repeat rewrite bi.wand_curry.
-    intantiateWand.
-    instWithPEvar taskPost.
-    go.
-    iSplitL "".
-    { verify_spec'.
-      go.
-      iExists _. eagerUnifyU.
-      autorewrite with syntactic. go.
-      erefl.
-    }
-    unhideAllFromWork. subst taskPost.
-    autorewrite with syntactic. go. 
-    iExists _. eagerUnifyU. 
-    autorewrite with syntactic. go.
-    wapply @arrayR_combinep. eagerUnifyU.
-    autorewrite with syntactic. go.
-    (* c++ semantics computes ... postcond requires *)
-    icancel (cancel_at p);[| go].
-    do 2 f_equiv.
-    symmetry.
-    apply fold_split_gcd.
-    auto.
-    Check fold_split.
-  Qed.
-  Lemma fold_split_gcd  (l: list Z) (pl: forall a, In a l -> 0 <= a) (lSplitSize: nat):
-    fold_left Z.gcd l 0=
-      Z.gcd (fold_left Z.gcd (firstn lSplitSize l) 0) (fold_left Z.gcd (skipn lSplitSize l) 0).
-  Proof using. apply misc.fold_split_gcd; auto. Qed.
-
-  (** *Structs and Classes
-     we often use multi-word numbers: EVMword is 256 bits *)
-  
-  Lemma unint32 (p:ptr) (v:Z) : p |-> primR uint 1 v |-- [| 0 <=v < 2^32 |] ** p |-> primR uint 1 v.
-  Proof.
-    go.
-  Qed.
-
-
-  
-  (*class UnboundUint *)
-  
-  Require Import Coq.NArith.BinNat.
-  Require Import Coq.Lists.List.
-  Require Import Coq.Wellfounded.Wellfounded.
-  Require Import Coq.Program.Wf.
-  Import ListNotations.
-  Require Import FunInd.
-
-  Open Scope N_scope.
-  Search N.size.
-  Require Import Recdef.
-  Function split_in_32 (n : N) {measure (fun n => N.to_nat (N.log2 n))} : list N :=
-    match n with
-    | 0%N => []
-    | 1%N => [1]
-    | _ =>
-        let chunk := n `mod` (2^32) in
-        let n'   := n / (2^32) in
-        chunk :: split_in_32 n'
-    end.
-  Proof.
-    {
-      intros. subst.
-      rewrite <- N.shiftr_div_pow2.
-      repeat rewrite N.log2_shiftr.
-      simpl.
-      lia.
-    }
-    {
-      intros. subst.
-      rewrite <- N.shiftr_div_pow2.
-      repeat rewrite N.log2_shiftr.
-      simpl.
-      lia.
-    }
-  Defined.
-
-  Eval vm_compute in (split_in_32 (2^65 + 2^32 + 45)).
-
-  Definition UnboundUintR (q:Qp) (n:N) : Rep :=
-    let pieces32 : list N := split_in_32 n in 
-    _field "size" |-> primR uint q (length pieces32)
-      ** Exists arrBase, _field "data" |-> primR uint q (Vptr arrBase)
-                           ** pureR (arrBase |-> arrayR uint (fun i:N => primR uint q i)  pieces32).
-  (** note the logical abstraction *)
-
-  Example unfoldUnboundUintR (p:ptr) q n:
-    let pieces32 := split_in_32 n in   
-    p |-> UnboundUintR q n -|-
-      p |-> _field "size" |-> primR uint q (length pieces32)
-      ** Exists arrBase, p |-> _field "data" |-> primR uint q (Vptr arrBase)
-                           ** arrBase |-> arrayR uint (fun i:N => primR uint q i)  pieces32.
-  Proof. simpl.  unfold UnboundUintR. iSplit; go. Qed.
-
-  Transparent atomicR.
-  
-  
-   (*
-    (λ this : ptr,
-       \arg{(Q : bool → mpred) (x : bool)} "v" (Vbool x)
-       \pre
-         AU1 << ∀ y : bool, this |-> atomicR Tbool (Vbool y) (cQp.mut 1) >> @ ⊤, ∅
-            << this |-> atomicR Tbool (Vbool x) (cQp.mut 1), COMM Q y >> 
-       \post{y : bool}[Vbool y]
-                Q y)
-  Rep ~= ptr -> mpred
-                *)
-
-  Locate inv.
+      
   Definition LockR (q: cQp.t) (invId: gname) (lockProtectedResource: mpred) : Rep :=
   as_Rep (fun (this:ptr)=>
      this |-> structR "::SpinLock" q
@@ -1087,16 +749,6 @@ also, arrays
          \pre R
          \post emp
       ).
-    #[ignore_errors]
-    cpp.spec "std::atomic<bool>::exchange(bool, enum std::memory_order)"  as exchange_spec with
-            (λ this : ptr,
-       \arg{(x : bool)} "v" (Vbool x)
-       \arg "order" (Vint memory_order_seq_cst)
-       \pre{Q : bool → mpred}
-         AC1 << ∀ y : bool, this |-> atomicR Tbool (cQp.mut 1) (Vbool y)>> @ ⊤, ∅
-            << this |-> atomicR Tbool (cQp.mut 1) (Vbool x), COMM Q y >> 
-       \post{y : bool}[Vbool y]
-       Q y).
     Opaque atomicR.
   
   Lemma lock_lock_prf: denoteModule module ** exchange_spec |-- lock_spec.
@@ -1107,7 +759,6 @@ also, arrays
     go.
     iExists (fun oldval:bool => (if oldval then emp else R) **  cinvq ns invId q
         (∃ locked : bool, this |-> o_field CU "SpinLock::locked" |-> atomicR "bool" 1%Qp (Vbool locked) ∗ (if locked then emp else R))).
-    Require Import bedrock.auto.tactics.
     wrename [cinvq _ _ _ _]  "inv".
     iSplitL "inv".
     -
@@ -1122,15 +773,6 @@ also, arrays
     - go.
       wp_if; go.
    Qed.
-    #[ignore_errors]
-    cpp.spec "std::atomic<bool>::store(bool, enum std::memory_order)"  as store_spec with
-(λ this : ptr,
-       \arg{(Q : mpred) (x : bool)} "v" (Vbool x)
-       \arg "memorder" (Vint 5)
-       \pre
-         AC1 << ∀ y : bool, this |-> atomicR Tbool (cQp.mut 1) (Vbool y)>> @ ⊤, ∅
-            << this |-> atomicR Tbool (cQp.mut 1) (Vbool x), COMM Q >> 
-                                                               \post    Q).
       
   Lemma unlock_prf: denoteModule module ** store_spec |-- unlock_spec.
   Proof using MODd.
@@ -1151,10 +793,10 @@ End with_Sigma.
 
 (* TODO:
 2: clean this file
-4. BlockState tikz aniimation
 8. narrartive+offsets in coments.
 7. lock protected linked list: code
 10. lock protected linked list: tikz animation
+11. fold_left proof w/ function ptr
 
 done:
 0. linkedlist
@@ -1164,6 +806,7 @@ done:
 5. counter auth frag specs
 9. spec of BlockState::read_storage
 6. BlockState::merge and can_merge specs: cleanup
+4. BlockState tikz aniimation
 
 
 sequence:
