monadproofs/proofs/misc.v
@@ -7,6 +7,37 @@ From AAC_tactics Require Import AAC.
 From AAC_tactics Require Import Instances.
 Import Instances.Z.
 Import cQp_compat.
+Lemma lose_resources `{cpp_logic} (P:mpred): P |-- emp.
+Proof using.
+  go.
+Qed.
+
+Lemma cinvq_alloc `{cpp_logic} (E : coPset) (N : namespace) (P : mpred) :
+  WeaklyObjective P → ▷ P |-- |={E}=> ∃ γ : gname, cinvq N γ 1 P.
+Proof.
+  intros.
+  unfold cinvq.
+  wapply (cinv_alloc E N P).
+  work.
+  iModIntro.
+  ework.
+  eagerUnifyU. go.
+Qed.
+
+Definition cQpc := cQp.mk false.
+Lemma mut_mut_add: ∀ q1 q2 : Qp, cQp.mut (q1 + q2) = (cQp.mut q1 + cQp.mut q2)%cQp.
+Proof. intros. reflexivity. Qed.
+
+  Ltac solveCqpeq :=
+    repeat match goal with
+        H:Qp |- _ => destruct H; simpl in *
+      end;
+      unfold cQpc, cQp.scale; simpl in *;
+      repeat rewrite <- mut_mut_add;
+       f_equal;              
+        solveQpeq;
+        solveQeq.
+
 Import linearity.
 Hint Rewrite @firstn_all: syntactic.
 Hint Rewrite Nat.add_0_r Z.add_0_r :syntactic.
@@ -158,10 +189,50 @@ Ltac wapplyObserve lemma:=
     || wapply (@observe_2_elim _ _ _ _ (lemma _ _ _ _ _ _ _ _)) || wapply (@observe_2_elim _ _ _ _ (lemma _ _ _ _ _ _ _ _ _))
     || wapply (@observe_2_elim _ _ _ _ (lemma _ _ _ _ _ _ _ _ _ _)) || wapply (@observe_2_elim _ _ _ _ (lemma _ _ _ _ _ _ _ _ _ _ _))
   ].
+Section tacLemmas.
+  Context `{Sigma:cpp_logic} {CU: genv} {hh: HasOwn mpredI algebra.frac.fracR}. (* some standard assumptions about the c++ logic *)
+  
+  Lemma observe_elim_rep (Q P : Rep) (p:ptr): Observe Q P → p |-> P ⊢ p|->(P ∗ Q).
+  Proof using.
+    intros Ho.
+    apply _at_mono.
+    wapplyObserve Ho.
+    go.
+  Qed.
+  
+  Lemma observe_2_elim_rep Q P1 P2 (p:ptr) {O : Observe2 Q P1 P2} : p|->P1 ⊢ p|-> P2 -∗ p|->P1 ∗ p|->P2 ∗ p|->Q.
+  Proof.
+    iIntros. iStopProof.
+    repeat rewrite <- _at_sep.
+    apply _at_mono.
+    wapplyObserve O.
+    go.
+  Qed.
+End tacLemmas.
+
+Ltac wapplyObserveRep lemma:=
+  try intros;
+  idtac;
+  [
+    wapply (@observe_elim_rep _ _ _ _ _ _ (lemma)) || wapply (@observe_elim_rep _ _ _ _ _ _ (lemma _))
+    || wapply (@observe_elim_rep _ _ _ _ _ _ (lemma _ _)) || wapply (@observe_elim_rep _ _ _ _ _ _ (lemma _ _ _))
+    || wapply (@observe_elim_rep _ _ _ _ _ _ (lemma _ _ _ _)) || wapply (@observe_elim_rep _ _ _ _ _ _ (lemma _ _ _ _ _))
+    || wapply (@observe_elim_rep _ _ _ _ _ _ (lemma _ _ _ _ _ _)) || wapply (@observe_elim_rep _ _ _ _ _ _ (lemma _ _ _ _ _ _ _))
+    || wapply (@observe_elim_rep _ _ _ _ _ _ (lemma _ _ _ _ _ _ _ _)) || wapply (@observe_elim_rep _ _ _ _ _ _ (lemma _ _ _ _ _ _ _ _ _))
+    || wapply (@observe_elim_rep _ _ _ _ _ _ (lemma _ _ _ _ _ _ _ _ _ _)) || wapply (@observe_elim_rep _ _ _ _ _ _ (lemma _ _ _ _ _ _ _ _ _ _ _))
+    
+    || wapply (@observe_2_elim_rep _ _ _ _ _ _ _ (lemma)) || wapply (@observe_2_elim_rep _ _ _ _ _ _ _ (lemma _))
+    || wapply (@observe_2_elim_rep _ _ _ _ _ _ _ (lemma _ _)) || wapply (@observe_2_elim_rep _ _ _ _ _ _ _ (lemma _ _ _))
+    || wapply (@observe_2_elim_rep _ _ _ _ _ _ _ (lemma _ _ _ _)) || wapply (@observe_2_elim_rep _ _ _ _ _ _ _ (lemma _ _ _ _ _))
+    || wapply (@observe_2_elim_rep _ _ _ _ _ _ _ (lemma _ _ _ _ _ _)) || wapply (@observe_2_elim_rep _ _ _ _ _ _ _ (lemma _ _ _ _ _ _ _))
+    || wapply (@observe_2_elim_rep _ _ _ _ _ _ _ (lemma _ _ _ _ _ _ _ _)) || wapply (@observe_2_elim_rep _ _ _ _ _ _ _ (lemma _ _ _ _ _ _ _ _ _))
+    || wapply (@observe_2_elim_rep _ _ _ _ _ _ _ (lemma _ _ _ _ _ _ _ _ _ _)) || wapply (@observe_2_elim_rep _ _ _ _ _ _ _ (lemma _ _ _ _ _ _ _ _ _ _ _))
+    
+  ].
 
 Section cp.
   Context `{Sigma:cpp_logic} {CU: genv} {hh: HasOwn mpredI algebra.frac.fracR}. (* some standard assumptions about the c++ logic *)
-
+  
   Definition parrayR  {T:Type} ty (Rs : nat -> T -> Rep) (l: list T) : Rep :=
   .[ ty ! length l ] |-> validR ** [| is_Some (size_of _ ty) |] **
   (* ^ both of these are only relevant for empty arrays, otherwise, they are implied by the
@@ -789,9 +860,134 @@ Section cp.
   Definition primR2_anyRC := [CANCEL] primR2_anyR.
   
   #[global] Instance learnArrUnsafe e t: LearnEq2 (@arrayR _ _ _ e _ t) := ltac:(solve_learnable).
+
+  Definition atomic_core_field_offset : offset. Proof. Admitted.
+  Definition atomicR (ty:type) (q : cQp.t) (v : val) : Rep :=
+    structR (Ninst "std::atomic" [Atype ty]) q
+    ** o_base CU (Ninst "std::atomic" [Atype ty]) (Ninst "std::__atomic_base" [Atype ty]) |-> structR  (Ninst "std::__atomic_base" [Atype ty]) q
+    ** atomic_core_field_offset |-> primR ty q v.
+
+(** Properties of [atomicR] *)
+Section atomicR.
+  Definition ns := (nroot .@@ "::SpinLock").
+
+  #[global] Instance atomicR_frac T : CFracSplittable_1 (atomicR T).
+  Proof.  solve_cfrac. Qed.
+
+  #[global] Instance atomic_type_ptrR_observe ty v q
+    : Observe (type_ptrR (Tnamed (Ninst "std::atomic" [Atype ty]))) (atomicR ty v q) := _.
+
+  #[global] Instance atomic_type_ptrR_base_observe ty v q (p:ptr)
+    : Observe (type_ptr (Tnamed (Ninst "std::__atomic_base" [Atype ty])) (p,, o_base CU (Ninst "std::atomic" [Atype ty]) (Ninst "std::__atomic_base" [Atype ty]))) (p |-> atomicR ty v q).
+  Proof.
+    apply observe_intro;[exact _|].
+    iIntrosDestructs.
+    unfold atomicR.
+    hideRhs.
+    go.
+    unhideAllFromWork.
+    go.
+  Qed.
   
+  #[global] Instance atomic_agree ty v1 v2 q1 q2
+    : Observe2 [| v1 = v2 |] (atomicR ty q1 v1) (atomicR ty q2 v2) := _.
+
+  #[global] Instance atomic_agree_inj `{Vinj : A -> val} `{!Inj eq eq Vinj} ty v1 v2 q1 q2
+    : Observe2 [| v1 = v2 |] (atomicR ty q1 (Vinj v1)) (atomicR ty q2 (Vinj v2)).
+  Proof. exact: (observe2_inj Vinj). Qed.
+
+  Definition learn_atomic_val (p : ptr) ty v1 v2 q1 q2
+    : Learnable (p |-> atomicR ty q1 v1) (p |-> atomicR ty q2 v2) [v2=v1].
+  Proof. solve_learnable. Qed.
+
+  Definition learn_atomic_val_UNSAFE (p : ptr) ty v1 v2 q1 q2
+    : Learnable (p |-> atomicR ty q1 v1) (p |-> atomicR ty q2 v2) [v2=v1; q1=q2].
+  Proof. solve_learnable. Qed.
+  (** [atomicR ty q v] implies that value [v] has type [ty]. *)
+  Lemma atomicR_has_type_prop ty v q :
+    Observe [| has_type_prop v ty |] (atomicR ty q v).
+  Proof. refine _. Qed.
+
+  Opaque atomicR.
+  Lemma atomicR_combine (p:ptr) (q1 q2: Qp) (v1 v2 : val) ty:
+    p |-> atomicR ty q1 v1 ** p |-> atomicR ty q2 v2
+      |-- p |-> atomicR ty (q1+q2) v1 ** [| v1 = v2 |].
+  Proof using.
+    go.
+    wapplyObserveRep atomic_agree. eagerUnifyU. go.
+    rewrite -> @cfractional.cfractional with (P := fun q => atomicR ty q v1);[| exact _].
+    go.
+  Qed.
+  Lemma atomicR_combine_half (p:ptr) (q: Qp) (v1 v2 : val) ty:
+    p |-> atomicR ty (q/2) v1 ** p |-> atomicR ty (q/2) v2
+      |-- p |-> atomicR ty q v1 ** [| v1 = v2 |].
+  Proof using.
+    rewrite atomicR_combine.
+    go.
+    iClear "#".
+    iStopProof.
+    apply _at_mono.
+    f_equiv.
+    solveCqpeq.
+  Qed.
+  Definition atomicR_combineF := [FWD] atomicR_combine.
+  
+End atomicR.
+
+  Definition fwd_later_exist := [FWD] (@bi.later_exist).
+  Definition fwd_later_sep := [FWD] (@bi.later_sep).
+  Definition bwd_later_exist := [BWD_MW->] (@bi.later_exist).
+  Definition bwd_later_sep := [BWD_MW->] (@bi.later_sep).
+  Definition fwd_at_later := [FWD<-] (@_at_later).
+
+  Lemma splitcinvq (P:mpred) ns (invId: gname) (q:Qp):
+    cinvq ns invId q P |-- cinvq ns invId (q/2) P ** cinvq ns invId (q/2) P.
+  Proof using.
+    rewrite <- (@fractional _ _ (cinvq_frac _)).
+    f_equiv.
+    solveCqpeq.
+  Qed.
+  Definition cinvqC := [CANCEL] splitcinvq.
+  
+    Opaque coPset_difference.
+
+    Lemma peek_cinvq a b c P (C:mpred) learn:
+      ▷ P |-- bupd (▷ P ** learn) 
+      -> (learn -* cinvq a b c P -*  |={⊤}=> C) |-- cinvq a b c P -*  |={⊤}=> C.
+    Proof using.
+      intros hl.
+      go.
+      openCinvq.
+      rewrite hl.
+      ghost.
+      go.
+      wapply invariants.close_cinvQR4.
+      eagerUnifyU.
+      unhideAllFromWork.
+      go.
+      iModIntro.
+      iFrame.
+    Qed.
+
+    Lemma admitReferenceTo ty ptr : emp |-- reference_to ty ptr.
+    Proof. Admitted.
+
+  Lemma atomicr_split (p:ptr) ty (q:Qp) v :
+    p|-> atomicR ty (cQp.mut q) v -|- (p |-> atomicR ty (cQp.mut q/2) v) ** p |-> atomicR ty (cQp.mut q/2) v.
+  Proof using.
+    rewrite -> cfractional_split_half with (R := fun q => atomicR ty q v);[| exact _].
+    rewrite _at_sep.
+    f_equiv; f_equiv; f_equiv;
+      solveCqpeq.
+  Qed.
+  Definition atomicrC := [CANCEL] atomicr_split.
+  Definition lcinvqg_unsafe a1 g1 q1 P1 a2 g2 q2 P2:
+    Learnable (cinvq a1 g1 q1 P1) (cinvq a2 g2 q2 P2) [g1=g2] := ltac:(solve_learnable).
+    
 End cp.
 Opaque parrayR.
+(*  Hint Resolve fwd_later_exist fwd_later_sep bwd_later_exist
+    bwd_later_sep : br_opacity. *)
 Lemma cancelLstar {PROP:bi} {T} l (va vb : T -> PROP):
   (forall id, id ∈ l -> va id |-- vb id) ->
   ([∗ list] id ∈ l, va id) |-- ([∗ list] id ∈ l,vb id).
@@ -897,3 +1093,71 @@ Ltac ren addr v :=
               addr |-> primR _ _ (Vint ?x) => rename x into v
             end
          ).
+Ltac lose_resources := try iStopProof; apply lose_resources.
+
+
+
+(* open all cinvq invariants then open rest. used in callAtomicCommitCinv*)
+Ltac openCinvqsRest :=
+  repeat openCinvq;
+  work using fwd_later_exist, fwd_later_sep;
+  repeat removeLater;
+  iApply fupd_mask_intro;[set_solver |]; (* openRest *)
+  iIntrosDestructs.
+
+(**
+   the RHS of your goal should look like a permutation of
+   [[
+   AC pre post ?Q ** (forall ..., ?Q ... -* ...)
+   ]]
+  it first calls [callAtomicCommit] to instantiate the public post Q.
+  then it opens all cinvq invariants
+  then it opens everything else (change the goal from [|={⊤ \ ..\ ... ,∅}=> U)] to  [|={∅}=> U)])
+  and then "does iModIntro" so that you can start proving U which is typically of the form [pre ** ...]
+ *)
+Ltac callAtomicCommitCinv :=
+  repeat (iExists _);
+  callAtomicCommit;
+  openCinvqsRest.
+
+(* applies to goals that look like [|-- AC pre post Q] or [|-- AU pre post Q]  in IPM: only 1 conjuct in conclusion and not 2, where [callAtomicCommitCinv] works. it sets up the proof of AC/AU by doing the usual initialization
+ and opening all invariants and rest so that you can immediately begin proving [pre] *)
+Ltac proveAuAc :=
+  (iAcIntro || iAuIntro);
+  (unfold commit_acc || unfold atomic_acc);
+  openCinvqsRest.
+
+Lemma cinvq_alloc_no_shared_pages `{Σ : cpp_logic} (E : coPset) (N : namespace) (P : mpred) :
+  ▷ P |-- |={E}=> ∃ γ : gname, cinvq N γ 1 P.
+  Proof.
+    intros.
+    apply cinvq_alloc.
+  Admitted. (* when there are no shared pages between processes, all C++ memory locations (ptr) are objective, else one has to look at the underlying physical address on the host machine *)
+  
+Notation uint := "unsigned int"%cpp_type.
+
+Ltac solveRefereceTo :=
+  IPM.perm_right ltac:(fun R _ =>
+                             match R with
+                             | reference_to ?ty ?p =>
+                                 wapply (admitReferenceTo ty p)
+                             end
+                      ).
+
+Lemma fold_id2 {A:Type} (f: A->A->A) (asoc: Associative (=) f)
+  (start id: A) (lid: LeftId (=) id f) (rid: RightId (=) id f) (l: list A):
+  fold_left f l start = f start (fold_left f l id).
+Proof using.
+  hnf in lid.
+  hnf in rid.
+  revert start.
+  induction l; auto.
+  simpl.
+  simpl. rewrite lid.
+  intros.
+  simpl.
+  rewrite IHl.
+  symmetry.
+  rewrite IHl.
+  aac_reflexivity.
+Qed.
