monadproofs/proofs/demo2prfb.v
@@ -1,0 +1,135 @@
+Require Import monad.proofs.demo2.
+Require Import bedrock.auto.invariants.
+Require Import bedrock.auto.cpp.proof.
+Require Import bedrock.auto.cpp.tactics4.
+
+Require Import monad.proofs.misc. (* monad/proofs/misc.v *)
+Require Import monad.proofs.demomisc.
+Require Import monad.proofs.demoprf.
+From AAC_tactics Require Import AAC.
+From AAC_tactics Require Import Instances.
+Import Instances.Z.
+Import stdpp.list.
+Import stdpp.decidable.
+Import cQp_compat.
+Open Scope cQp_scope.
+Open Scope Z_scope.
+Import Verbose.
+Disable Notation take.
+Disable Notation drop.
+Disable Notation "`div`" (all).
+Disable Notation intR.
+Disable Notation uintR.
+
+Import linearity.
+Section with_Sigma.
+  Context `{Sigma:cpp_logic}  {CU: genv}.
+  Context  {MODd : demo2.module ⊧ CU}.
+
+  Lemma unint32 (p:ptr) (v:Z) : p |-> primR uint 1 v |-- [| 0 <=v < 2^32 |] ** p |-> primR uint 1 v.
+  Proof.
+    go.
+  Qed.
+
+
+  
+  (*class UnboundUint *)
+  
+  Require Import Coq.NArith.BinNat.
+  Require Import Coq.Lists.List.
+  Require Import Coq.Wellfounded.Wellfounded.
+  Require Import Coq.Program.Wf.
+  Import ListNotations.
+  Require Import FunInd.
+
+  Open Scope N_scope.
+  Search N.size.
+  Require Import Recdef.
+  Function split_in_32 (n : N) {measure (fun n => N.to_nat (N.log2 n))} : list N :=
+    match n with
+    | 0%N => []
+    | 1%N => [1]
+    | _ =>
+        let chunk := n `mod` (2^32) in
+        let n'   := n / (2^32) in
+        chunk :: split_in_32 n'
+    end.
+  Proof.
+    {
+      intros. subst.
+      rewrite <- N.shiftr_div_pow2.
+      repeat rewrite N.log2_shiftr.
+      simpl.
+      lia.
+    }
+    {
+      intros. subst.
+      rewrite <- N.shiftr_div_pow2.
+      repeat rewrite N.log2_shiftr.
+      simpl.
+      lia.
+    }
+  Defined.
+
+  Eval vm_compute in (split_in_32 (2^65 + 2^32 + 45)).
+
+  Definition UnboundUintR (q:Qp) (n:N) : Rep :=
+    let pieces32 : list N := split_in_32 n in 
+    _field "size" |-> primR uint q (length pieces32)
+      ** Exists arrBase, _field "data" |-> primR uint q (Vptr arrBase)
+                           ** pureR (arrBase |-> arrayR uint (fun i:N => primR uint q i)  pieces32).
+  (** note the logical abstraction *)
+
+  Example unfoldUnboundUintR (p:ptr) q n:
+    let pieces32 := split_in_32 n in   
+    p |-> UnboundUintR q n -|-
+      p |-> _field "size" |-> primR uint q (length pieces32)
+      ** Exists arrBase, p |-> _field "data" |-> primR uint q (Vptr arrBase)
+                           ** arrBase |-> arrayR uint (fun i:N => primR uint q i)  pieces32.
+  Proof. simpl.  unfold UnboundUintR. iSplit; go. Qed.
+
+  Definition AWrapperR  (q: Qp) (invId: gname): Rep :=
+    structR "AWRapper" q **
+    as_Rep (fun this:ptr =>
+      cinv invId q (∃ i:Z, this ,, _field "v" |-> atomicR "int" 1 i)).
+
+  (** above, i is ∃ quantified *)
+  Definition AWrapperRs  (q: Qp) (i:Z): Rep :=
+    structR "AWRapper" q **
+      _field "v" |-> atomicR "int" q (Vint i).
+
+  
+  cpp.spec "AWrapper::setValue(int)" as setValue_spec with (fun (this:ptr) =>
+     \prepost{q invid} this |-> AWrapperR q invid
+     \arg{newval:Z} "value" (Vint newval)
+     \post emp).
+  
+  cpp.spec "AWrapper::setValue(int)" as setValue_nonconcurrent_spec with (fun (this:ptr) =>
+     \pre{oldVal} this |-> AWrapperRs 1 oldVal
+     \arg{i:Z} "value" (Vint i)
+     \post this |-> AWrapperRs 1 i). (** but.. no other thread can call any method during this call *)
+
+  cpp.spec "AWrapper::getValue()" as getValue_spec with (fun (this:ptr) =>
+     \prepost{q invid} this |-> AWrapperR q invid
+     \post{any:Z} [Vint any] emp).
+
+  cpp.spec "AWrapper::getValue()" as getValue_nonconcurrent_spec with (fun (this:ptr) =>
+     \prepost{q (val:Z)} this |-> AWrapperRs q val
+     \post [Vint val] emp).
+  Definition AWrapperR2  (q: Qp) (invId: gname): Rep :=
+    structR "AWRapper" q **
+    as_Rep (fun this:ptr =>
+       cinv invId q (∃ i:Z, this ,, _field "v" |-> atomicR "int" 1 i
+                        ** [| isPrime i |] )).
+
+  cpp.spec "AWrapper::setValue(int)" as setValue2_spec with (fun (this:ptr) =>
+     \prepost{q invId} this |-> AWrapperR2 q invId
+     \arg{i:Z} "value" (Vint i)
+     \pre [| isPrime i |] 
+     \post emp).
+
+  cpp.spec "AWrapper::getValue()" as getValue2_spec with (fun (this:ptr) =>
+     \prepost{q invid} this |-> AWrapperR2 q invid
+     \post{any:Z} [Vint any] [| isPrime any |]).
+  
+End with_Sigma.
